concurrency/hack-hash-table/MapSpec.s.dfy
@@ -26,7 +26,7 @@ module MapIfc refines InputOutputIfc {
 
   datatype Output =
     | QueryOutput(res: QueryResult)
-    | InsertOutput
+    | InsertOutput(success: bool) // an insert may fail when there is no capacity
     | RemoveOutput(existed: bool) // to Travis: added the possibility that there is nothing to remove
 }
 
@@ -59,8 +59,15 @@ module MapSpec {
             && (key in s.m ==> output == Ifc.QueryOutput(Found(s.m[key])))
             && (key !in s.m ==> output == Ifc.QueryOutput(NotFound))
           case InsertInput(key, value) =>
-            && s'.m == s.m[key := value]
-            && output == Ifc.InsertOutput
+           (
+            && s' == s.(m := s.m[key := value])
+            && output == Ifc.InsertOutput(true)
+           )
+           ||
+           (
+            && s' == s
+            && output == Ifc.InsertOutput(false)
+           )
           case RemoveInput(key) =>
             && s'.m == s.m - {key}
             && output == Ifc.RemoveOutput(key in s.m)
